

TABLE I. Rewrite rules.

Class	Rewrite Rule	Instruction
Logical Operations	$(\text{And } ?a (\text{Or } ?a ?b)) \rightarrow ?a$	$A \wedge (A \vee B) = A$
	$(\text{And } ?b (\text{Or } ?a ?b)) \rightarrow ?b$	$B \wedge (A \vee B) = B$
	$(\text{Or } ?a (\text{And } ?a ?b)) \rightarrow ?a$	$A \vee (A \wedge B) = A$
	$(\text{Or } ?b (\text{And } ?a ?b)) \rightarrow ?b$	$B \vee (A \wedge B) = B$
	$(\text{Or } ?a ?a) \rightarrow ?a$	$A \vee A = A$
	$(\text{And } ?a ?a) \rightarrow ?a$	$A \wedge A = A$
	$(\text{Not } (\text{Not } ?a)) \rightarrow ?a$	$\neg(\neg A) = A$
	$(\text{Or } ?a ?b) \rightarrow (\text{Or } ?b ?a)$	$A \vee B = B \vee A$
	$(\text{And } ?a ?b) \rightarrow (\text{And } ?b ?a)$	$A \wedge B = B \wedge A$
	$(\text{Or } ?a (\text{Not } ?a)) \rightarrow \text{true}$	$A \vee \neg A = \text{true}$
	$(\text{Or } ?a \text{true}) \rightarrow \text{true}$	$A \vee \text{true} = \text{true}$
	$(\text{Or } ?a \text{false}) \rightarrow ?a$	$A \vee \text{false} = A$
	$(\text{And } ?a \text{true}) \rightarrow ?a$	$A \wedge \text{true} = A$
	$(\text{And } ?a \text{false}) \rightarrow \text{false}$	$A \wedge \text{false} = \text{false}$
	$(\text{And } (\text{Not } ?a) ?a) \rightarrow \text{false}$	$\neg A \wedge A = \text{false}$
Arithmetic Operations	$(\text{Add } ?a ?b) \rightarrow (\text{Add } ?b ?a)$	$A + B = B + A$
	$(\text{Add } ?a (\text{Add } ?b ?c)) \rightarrow (\text{Add } (\text{Add } ?a ?c) ?b)$	$A + (B + C) = (A + C) + B$
	$(\text{Mul } ?a ?b) \rightarrow (\text{Mul } ?b ?a)$	$A \times B = B \times A$
	$(\text{Mul } ?a (\text{Mul } ?b ?c)) \rightarrow (\text{Mul } (\text{Mul } ?a ?b) ?c)$	$A \times (B \times C) = (A \times B) \times C$
	$(\text{Add } (\text{Mul } ?a ?b) (\text{Mul } ?a ?c)) \rightarrow (\text{Mul } ?a (\text{Add } ?b ?c))$	$A \times B + A \times C = A \times (B + C)$
	$(\text{Add } (\text{Mul } ?a ?c) (\text{Mul } ?b ?c)) \rightarrow (\text{Mul } ?c (\text{Add } ?a ?b))$	$A \times C + B \times C = C \times (A + B)$
	$(\text{Add } ?a (\text{Sub } (\text{Atom } (\text{Int } 0)) ?b)) \rightarrow (\text{Sub } ?a ?b)$	$A + (0 - B) = A - B$
	$(\text{Div } (\text{Div } ?a ?b) ?c) \rightarrow (\text{Div } (\text{Div } ?a ?c) ?b)$	$(A \div B) \div C = (A \div C) \div B$
	$(\text{Div } ?a ?b) \rightarrow (\text{Mul } ?a (\text{Div } (\text{Atom } (\text{Int } 1)) ?b))$	$A \div B = A \times (1 \div B)$
	$(\text{Div } ?a (\text{Mul } ?b ?c)) \rightarrow (\text{Div } (\text{Div } ?a ?b) ?c)$	$A \div (B \times C) = (A \div B) \div C$
	$(\text{Mod } (\text{Add } ?a ?b) ?c) \rightarrow (\text{Mod } (\text{Add } (\text{Mod } ?a ?c) (\text{Mod } ?b ?c)) ?c)$	$(A + B) \bmod C = ((A \bmod C) + (B \bmod C)) \bmod C$
	$(\text{Mod } (\text{Sub } ?a ?b) ?c) \rightarrow (\text{Mod } (\text{Sub } (\text{Mod } ?a ?c) (\text{Mod } ?b ?c)) ?c)$	$(A - B) \bmod C = ((A \bmod C) - (B \bmod C)) \bmod C$
	$(\text{Mod } (\text{Mul } ?a ?b) ?c) \rightarrow (\text{Mod } (\text{Mul } (\text{Mod } ?a ?c) (\text{Mod } ?b ?c)) ?c)$	$(A \times B) \bmod C = ((A \bmod C) \times (B \bmod C)) \bmod C$
	$(\text{Mod } (\text{Power } ?a ?b) ?c) \rightarrow (\text{Mod } (\text{Power } (\text{Mod } ?a ?c) (\text{Mod } ?b ?c)) ?c)$	$(A^B) \bmod C = ((A \bmod C)^{B \bmod C}) \bmod C$
	$(\text{Mod } (\text{Add } (\text{Mod } (\text{Add } ?a ?b) ?c) ?d) ?c) \rightarrow$ $(\text{Mod } (\text{Add } ?a (\text{Mod } (\text{Add } ?b ?d) ?c) ?c))$	$((A + B) \bmod C) \bmod C = (A + ((B + D) \bmod C)) \bmod C$
	$(\text{Mod } (\text{Mul } (\text{Mod } (\text{Mul } ?a ?b) ?c) ?d) ?c) \rightarrow$ $(\text{Mod } (\text{Mul } ?a (\text{Mod } (\text{Mul } ?b ?d) ?c) ?c))$	$((A \times B) \bmod C) \bmod C = (A \times ((B \times D) \bmod C)) \bmod C$
	$(\text{Mod } (\text{Mul } (\text{Mod } (\text{Add } ?a ?b) ?c) ?d) ?c) \rightarrow$ $(\text{Mod } (\text{Add } (\text{Mod } (\text{Mul } ?a ?d) ?c) (\text{Mod } (\text{Mul } ?b ?d) ?c) ?c))$	$((A + B) \bmod C) \bmod C = ((A \times D \bmod C) + (B \times D \bmod C)) \bmod C$
	$(\text{Add } ?a ?a) \rightarrow (\text{Mul } ?a (\text{Atom } (\text{Int } 2)))$	$A + A = A \times 2$
	$(\text{Mul } ?a ?a) \rightarrow (\text{Power } ?a (\text{Atom } (\text{Int } 2)))$	$A \times A = A^2$
	$(\text{Add } ?a (\text{Atom } (\text{Int } 0))) \rightarrow ?a$	$A + 0 = A$
	$(\text{Sub } ?a (\text{Atom } (\text{Int } 0))) \rightarrow ?a$	$A - 0 = A$
	$(\text{Sub } (\text{Atom } (\text{Int } 0)) ?a) \rightarrow (\text{Subone } ?a)$	$0 - A = -A$
	$(\text{Mul } ?a (\text{Atom } (\text{Int } 0))) \rightarrow (\text{Atom } (\text{Int } 0))$	$A \times 0 = 0$
	$(\text{Mul } ?a (\text{Atom } (\text{Int } 1))) \rightarrow ?a$	$A \times 1 = A$
	$(\text{Div } (\text{Atom } (\text{Int } 0)) ?a) \rightarrow (\text{Atom } (\text{Int } 0))$	$0 \div A = 0$
	$(\text{Div } ?a (\text{Atom } (\text{Int } 1))) \rightarrow ?a$	$A \div 1 = A$
	$(\text{Mod } ?a (\text{Atom } (\text{Int } 1))) \rightarrow (\text{Atom } (\text{Int } 0))$	$A \bmod 1 = 0$
	$(\text{Power } ?a (\text{Atom } (\text{Int } 0))) \rightarrow (\text{Atom } (\text{Int } 1))$	$A^0 = 1$
	$(\text{Power } ?a (\text{Atom } (\text{Int } 1))) \rightarrow ?a$	$A^1 = A$
Bitwise Operations	$(\text{BitAnd } ?a (\text{BitOr } ?a ?b)) \rightarrow ?a$	$A \& (A B) = A$
	$(\text{BitAnd } ?b (\text{BitOr } ?a ?b)) \rightarrow ?b$	$B \& (A B) = B$
	$(\text{BitOr } ?a (\text{BitAnd } ?a ?b)) \rightarrow ?a$	$A (A \& B) = A$
	$(\text{BitOr } ?b (\text{BitAnd } ?a ?b)) \rightarrow ?b$	$B (A \& B) = B$
	$(\text{BitOr } ?a ?a) \rightarrow ?a$	$A A = A$
	$(\text{BitAnd } ?a ?a) \rightarrow ?a$	$A \& A = A$
	$(\text{BitOr } ?a ?b) \rightarrow (\text{BitOr } ?b ?a)$	$A B = B A$
	$(\text{BitAnd } ?a ?b) \rightarrow (\text{BitAnd } ?b ?a)$	$A \& B = B \& A$
	$(\text{BitXor } ?a ?b) \rightarrow (\text{BitXor } ?b ?a)$	$A \oplus B = B \oplus A$
Associative/ Distributive	$(\text{BitOr } (\text{BitOr } ?a ?b) ?c) \rightarrow (\text{BitOr } ?a (\text{BitOr } ?b ?c))$	$(A B) C = A (B C)$
	$(\text{BitAnd } (\text{BitAnd } ?a ?b) ?c) \rightarrow (\text{BitAnd } ?a (\text{BitAnd } ?b ?c))$	$(A \& B) \& C = A \& (B \& C)$
	$(\text{BitAnd } ?a (\text{BitOr } ?b ?c)) \rightarrow (\text{BitOr } (\text{BitAnd } ?a ?b) (\text{BitAnd } ?a ?c))$	$A \& (B C) = (A \& B) (A \& C)$
	$(\text{BitOr } ?a (\text{BitAnd } ?b ?c)) \rightarrow (\text{BitAnd } (\text{BitOr } ?a ?b) (\text{BitOr } ?a ?c))$	$A (B \& C) = (A B) \& (A C)$
Shift Operations	$(\text{Mul } (\text{Power } (\text{Atom } (\text{Int } 2)) ?b) ?a) \rightarrow (\text{ShiftLeft } ?a ?b)$	$2^B * A = A \ll B$
	$(\text{ShiftLeft } ?a (\text{Add } ?b ?c)) \rightarrow (\text{ShiftLeft } (\text{ShiftLeft } ?a ?b) ?c)$	$A \ll (B + C) = (A \ll B) \ll C$
	$(\text{Mul } ?a 2) \rightarrow (\text{shiftLeft } ?a (\text{Atom } (\text{Int } 1)))$	$A * 2 = A \ll 1$
	$(\text{ShiftLeft } (\text{Mul } ?a ?b) ?c) \rightarrow (\text{Mul } (\text{ShiftLeft } ?a ?c) ?b)$	$(A \times B) \ll C = (A \ll C) \times B$
	$(\text{AshiftLeft } (\text{Mul } ?a ?b) ?c) \rightarrow (\text{Mul } (\text{AshiftLeft } ?a ?c) ?b)$	$(A \times B) \lll C = (A \lll C) \times B$
	$(\text{Mul } (\text{Power } (\text{Atom } (\text{Int } 2)) ?b) ?a) \rightarrow (\text{AshiftLeft } ?a ?b)$	$A \times 2^B = A \lll B$
	$(\text{AshiftLeft } ?a (\text{Add } ?b ?c)) \rightarrow (\text{AshiftLeft } (\text{AshiftLeft } ?a ?b) ?c)$	$A \lll (B + C) = (A \lll B) \lll C$
	$(\text{Mul } ?a (\text{Atom } (\text{Int } 2))) \rightarrow (\text{AshiftLeft } ?a (\text{Atom } (\text{Int } 1)))$	$A \times 2 = A \lll 1$
	$(\text{Mul } (\text{ShiftLeft } ?a ?c) ?b) \rightarrow (\text{ShiftLeft } (\text{Mul } ?a ?b) ?c)$	$(A \ll C) \times B = (A \times B) \ll C$
	$(\text{Mul } (\text{AshiftLeft } ?a ?c) ?b) \rightarrow (\text{AshiftLeft } (\text{Mul } ?a ?b) ?c)$	$(A \lll C) \times B = (A \times B) \lll C$
	$(\text{Div } ?a (\text{Power } 2 ?b)) \rightarrow (\text{ShiftRight } ?a ?b)$	$A \div 2^B = A \gg B$
	$(\text{ShiftRight } (\text{ShiftRight } ?a ?b) ?c) \rightarrow (\text{ShiftRight } ?a (\text{Add } ?b ?c))$	$(A \gg B) \gg C = A \gg (B + C)$
	$(\text{Mul } ?a (\text{Power } 2 ?b)) \rightarrow (\text{ShiftLeft } ?a ?b)$	$A \times 2^B = A \ll B$
	$(\text{AshiftRight } ?a (\text{Add } ?b ?c)) \rightarrow (\text{AshiftRight } (\text{AshiftRight } ?a ?b) ?c)$	$(A \ggg B) \ggg C = A \ggg (B + C)$
	$(\text{Div } ?a (\text{Atom } (\text{Int } 2))) \rightarrow (\text{ShiftRight } ?a (\text{Atom } (\text{Int } 1)))$	$A \div 2 = A \gg 1$
	$(\text{BitAnd } (\text{ShiftRight } ?a ?b) (\text{Atom } (\text{Int } 1))) \rightarrow (\text{BitIndex } ?a ?b)$	$(A \gg B) \& 1 = A[B]$
	$(\text{Mul } (\text{ShiftRight } ?a ?c) ?b) \rightarrow (\text{ShiftRight } (\text{Mul } ?a ?b) ?c)$	$(A \gg C) \times B = (A \times B) \gg C$
	$(\text{Mul } (\text{AshiftRight } ?a ?c) ?b) \rightarrow (\text{AshiftRight } (\text{Mul } ?a ?b) ?c)$	$(A \ggg C) \times B = (A \times B) \ggg C$